James C - made stack evaluation inductive rather than functional

FlatStack/FlatStackLanguage.thy
@@ -11,23 +11,21 @@ type_synonym flat_stack_program = "code_label \<rightharpoonup> flat_stack_instr
 type_synonym flat_stack_state = "int list \<times> flat_stack_instruction list \<times> code_label \<times> output" 
   (* \<sigma>, \<pi>, s, \<omega> *)
 
-fun eval_flat_stack :: "flat_stack_program \<Rightarrow> flat_stack_state \<Rightarrow> flat_stack_state option" where
-  "eval_flat_stack \<Pi> (\<sigma>, [], s, \<omega>) = (case \<Pi> s of
-      Some (\<pi>, s') \<Rightarrow> Some (\<sigma>, \<pi>, s', \<omega>)
-    | None \<Rightarrow> None)"
-| "eval_flat_stack \<Pi> (i1 # i2 # \<sigma>, FAdd # \<pi>, s, \<omega>) = Some ((i2 + i1) # \<sigma>, \<pi>, s, \<omega>)"
-| "eval_flat_stack \<Pi> (i1 # i2 # \<sigma>, FSub # \<pi>, s, \<omega>) = Some ((i2 - i1) # \<sigma>, \<pi>, s, \<omega>)"
-| "eval_flat_stack \<Pi> (i1 # \<sigma>, FNeg # \<pi>, s, \<omega>) = Some ((-i1) # \<sigma>, \<pi>, s, \<omega>)"
-| "eval_flat_stack \<Pi> (i1 # i2 # \<sigma>, FEq # \<pi>, s, \<omega>) = Some (unboolify (i2 = i1) # \<sigma>, \<pi>, s, \<omega>)"
-| "eval_flat_stack \<Pi> (i1 # i2 # \<sigma>, FGt # \<pi>, s, \<omega>) = Some (unboolify (i2 > i1) # \<sigma>, \<pi>, s, \<omega>)"
-| "eval_flat_stack \<Pi> (i1 # i2 # \<sigma>, FLt # \<pi>, s, \<omega>) = Some (unboolify (i2 < i1) # \<sigma>, \<pi>, s, \<omega>)"
-| "eval_flat_stack \<Pi> (i1 # i2 # \<sigma>, FAnd # \<pi>, s, \<omega>) = 
-    Some (unboolify (boolify i2 \<and> boolify i1) # \<sigma>, \<pi>, s, \<omega>)"
-| "eval_flat_stack \<Pi> (i1 # i2 # \<sigma>, FOr # \<pi>, s, \<omega>) = 
-    Some (unboolify (boolify i2 \<or> boolify i1) # \<sigma>, \<pi>, s, \<omega>)"
-| "eval_flat_stack \<Pi> (i1 # \<sigma>, FNot # \<pi>, s, \<omega>) = Some (unboolify (\<not> boolify i1) # \<sigma>, \<pi>, s, \<omega>)"
-| "eval_flat_stack \<Pi> (i1 # \<sigma>, FPrint # \<pi>, s, \<omega>) = Some (\<sigma>, \<pi>, s, i1 # \<omega>)"
-| "eval_flat_stack \<Pi> \<Sigma> = None"
+inductive eval_flat_stack :: "flat_stack_program \<Rightarrow> flat_stack_state \<Rightarrow> flat_stack_state \<Rightarrow> bool" where
+  evf_jump [simp]: "\<Pi> s = Some (\<pi>, s') \<Longrightarrow> eval_flat_stack \<Pi> (\<sigma>, [], s, \<omega>) (\<sigma>, \<pi>, s', \<omega>)"
+| evf_add [simp]: "eval_flat_stack \<Pi> (i1 # i2 # \<sigma>, FAdd # \<pi>, s, \<omega>) ((i2 + i1) # \<sigma>, \<pi>, s, \<omega>)"
+| evf_sub [simp]: "eval_flat_stack \<Pi> (i1 # i2 # \<sigma>, FSub # \<pi>, s, \<omega>) ((i2 - i1) # \<sigma>, \<pi>, s, \<omega>)"
+| evf_neg [simp]: "eval_flat_stack \<Pi> (i1 # \<sigma>, FNeg # \<pi>, s, \<omega>) ((-i1) # \<sigma>, \<pi>, s, \<omega>)"
+| evf_eq [simp]: "eval_flat_stack \<Pi> (i1 # i2 # \<sigma>, FEq # \<pi>, s, \<omega>) (unboolify (i2 = i1) # \<sigma>, \<pi>, s, \<omega>)"
+| evf_gt [simp]: "eval_flat_stack \<Pi> (i1 # i2 # \<sigma>, FGt # \<pi>, s, \<omega>) (unboolify (i2 > i1) # \<sigma>, \<pi>, s, \<omega>)"
+| evf_lt [simp]: "eval_flat_stack \<Pi> (i1 # i2 # \<sigma>, FLt # \<pi>, s, \<omega>) (unboolify (i2 < i1) # \<sigma>, \<pi>, s, \<omega>)"
+| evf_and [simp]: "eval_flat_stack \<Pi> (i1 # i2 # \<sigma>, FAnd # \<pi>, s, \<omega>) 
+    (unboolify (boolify i2 \<and> boolify i1) # \<sigma>, \<pi>, s, \<omega>)"
+| evf_or [simp]: "eval_flat_stack \<Pi> (i1 # i2 # \<sigma>, FOr # \<pi>, s, \<omega>) 
+    (unboolify (boolify i2 \<or> boolify i1) # \<sigma>, \<pi>, s, \<omega>)"
+| evf_not [simp]: "eval_flat_stack \<Pi> (i1 # \<sigma>, FNot # \<pi>, s, \<omega>) 
+    (unboolify (\<not> boolify i1) # \<sigma>, \<pi>, s, \<omega>)"
+| evf_print [simp]: "eval_flat_stack \<Pi> (i1 # \<sigma>, FPrint # \<pi>, s, \<omega>) (\<sigma>, \<pi>, s, i1 # \<omega>)"
 
 fun flat_stack_output :: "flat_stack_state \<Rightarrow> output" where
   "flat_stack_output (\<sigma>, \<pi>, s, \<omega>) = \<omega>"
