Stack/StackLanguage.thy
@@ -15,21 +15,18 @@ datatype stack_value =
 type_synonym stack_state = "stack_value list \<times> stack_instruction list \<times> code_label \<times> output" 
   (* \<sigma>, \<pi>, s, \<omega> *)
 
-fun eval_stack :: "stack_program \<Rightarrow> stack_state \<Rightarrow> stack_state option" where
-  "eval_stack \<Pi> (\<sigma>, [], s, \<omega>) = (case \<Pi> s of
-      Some (\<pi>, s') \<Rightarrow> Some (\<sigma>, \<pi>, s', \<omega>)
-    | None \<Rightarrow> None)"
-| "eval_stack \<Pi> (IntV i1 # IntV i2 # \<sigma>, Add # \<pi>, s, \<omega>) = Some (IntV (i2 + i1) # \<sigma>, \<pi>, s, \<omega>)"
-| "eval_stack \<Pi> (IntV i1 # IntV i2 # \<sigma>, Sub # \<pi>, s, \<omega>) = Some (IntV (i2 - i1) # \<sigma>, \<pi>, s, \<omega>)"
-| "eval_stack \<Pi> (IntV i1 # \<sigma>, Neg # \<pi>, s, \<omega>) = Some (IntV (-i1) # \<sigma>, \<pi>, s, \<omega>)"
-| "eval_stack \<Pi> (IntV i1 # IntV i2 # \<sigma>, Eq # \<pi>, s, \<omega>) = Some (Bool (i2 = i1) # \<sigma>, \<pi>, s, \<omega>)"
-| "eval_stack \<Pi> (IntV i1 # IntV i2 # \<sigma>, Gt # \<pi>, s, \<omega>) = Some (Bool (i2 > i1) # \<sigma>, \<pi>, s, \<omega>)"
-| "eval_stack \<Pi> (IntV i1 # IntV i2 # \<sigma>, Lt # \<pi>, s, \<omega>) = Some (Bool (i2 < i1) # \<sigma>, \<pi>, s, \<omega>)"
-| "eval_stack \<Pi> (Bool i1 # Bool i2 # \<sigma>, And # \<pi>, s, \<omega>) = Some (Bool (i2 \<and> i1) # \<sigma>, \<pi>, s, \<omega>)"
-| "eval_stack \<Pi> (Bool i1 # Bool i2 # \<sigma>, Or # \<pi>, s, \<omega>) = Some (Bool (i2 \<or> i1) # \<sigma>, \<pi>, s, \<omega>)"
-| "eval_stack \<Pi> (Bool i1 # \<sigma>, Not # \<pi>, s, \<omega>) = Some (Bool (\<not> i1) # \<sigma>, \<pi>, s, \<omega>)"
-| "eval_stack \<Pi> (IntV i1 # \<sigma>, Print # \<pi>, s, \<omega>) = Some (\<sigma>, \<pi>, s, i1 # \<omega>)"
-| "eval_stack \<Pi> \<Sigma> = None"
+inductive eval_stack :: "stack_program \<Rightarrow> stack_state \<Rightarrow> stack_state \<Rightarrow> bool" where
+  evs_jump [simp]: "\<Pi> s = Some (\<pi>, s') \<Longrightarrow> eval_stack \<Pi> (\<sigma>, [], s, \<omega>) (\<sigma>, \<pi>, s', \<omega>)"
+| evs_add [simp]: "eval_stack \<Pi> (IntV i1 # IntV i2 # \<sigma>, Add # \<pi>, s, \<omega>) (IntV (i2 + i1) # \<sigma>, \<pi>, s, \<omega>)"
+| evs_sub [simp]: "eval_stack \<Pi> (IntV i1 # IntV i2 # \<sigma>, Sub # \<pi>, s, \<omega>) (IntV (i2 - i1) # \<sigma>, \<pi>, s, \<omega>)"
+| evs_neg [simp]: "eval_stack \<Pi> (IntV i1 # \<sigma>, Neg # \<pi>, s, \<omega>) (IntV (-i1) # \<sigma>, \<pi>, s, \<omega>)"
+| evs_eq [simp]: "eval_stack \<Pi> (IntV i1 # IntV i2 # \<sigma>, Eq # \<pi>, s, \<omega>) (Bool (i2 = i1) # \<sigma>, \<pi>, s, \<omega>)"
+| evs_gt [simp]: "eval_stack \<Pi> (IntV i1 # IntV i2 # \<sigma>, Gt # \<pi>, s, \<omega>) (Bool (i2 > i1) # \<sigma>, \<pi>, s, \<omega>)"
+| evs_lt [simp]: "eval_stack \<Pi> (IntV i1 # IntV i2 # \<sigma>, Lt # \<pi>, s, \<omega>) (Bool (i2 < i1) # \<sigma>, \<pi>, s, \<omega>)"
+| evs_and [simp]: "eval_stack \<Pi> (Bool i1 # Bool i2 # \<sigma>, And # \<pi>, s, \<omega>) (Bool (i2 \<and> i1) # \<sigma>, \<pi>, s, \<omega>)"
+| evs_or [simp]: "eval_stack \<Pi> (Bool i1 # Bool i2 # \<sigma>, Or # \<pi>, s, \<omega>) (Bool (i2 \<or> i1) # \<sigma>, \<pi>, s, \<omega>)"
+| evs_not [simp]: "eval_stack \<Pi> (Bool i1 # \<sigma>, Not # \<pi>, s, \<omega>) (Bool (\<not> i1) # \<sigma>, \<pi>, s, \<omega>)"
+| evs_print [simp]: "eval_stack \<Pi> (IntV i1 # \<sigma>, Print # \<pi>, s, \<omega>) (\<sigma>, \<pi>, s, i1 # \<omega>)"
 
 fun stack_output :: "stack_state \<Rightarrow> output" where
   "stack_output (\<sigma>, \<pi>, s, \<omega>) = \<omega>"
